\documentclass[./some_latex_template.tex]{subfiles}
\begin{document}

\title{Random Graph theory}
\author{Benjamin Chu}
\maketitle

\singlespacing
Most materials from this note is taken from \cite{Acemoglu, Ramchandran}

\section{Erdos-Renyi Graph Model}

\begin{itemize}
	\item We use $G(n, p)$ to denote an undirected (Erdos-Renyi) graph with $n$ nodes.
	\item An edge is formed between 2 nodes with probability $p \in (0, 1)$ \textbf{independently} of other edges. 
	\item A graph is \textbf{connected} when there is a path between every pair of vertices. 
\end{itemize}

\noindent When $p = p(n)$ is a function of $n$, we may be interested in the behavior of $G(n, p(n))$ as $n \rightarrow \infty$. 

\subsection{Warm-up}

\textbf{Q1. What is the probability that a vertex is isolated in $G(n, p)$?} \textbf{Ans:} A given node $i$ cannot form an edge with each of the remaining $n - 1$ nodes. Thus the probability is $(1 - p)^{n-1}$. 

\noindent \textbf{Q2. What is the probability that node 1 and node 2 are both isolated?} Let $I_1, I_2$ be the indicator that node 1 and node 2 are isolated. Then $P(I_1 \cap I_2) = P(I_1)P(I_2 \ | \ I_1)  = (1-p)^{n-1} * (1 - p)^{n - 2} = (1 - p)^{2n-3}$. 

\noindent \textbf{Q3. What is the probability that a group of $k$ nodes do not connect to the rest of the $n-k$ nodes?} There are ${n \choose k}$ number of ways to choose $k$ vertices. Each of these cannot form an edge with the remaining $n-k$ nodes independently with probability $(1-p)^{n-k}$. So overall we have $(1-p)^{(n-k)k}$. 

\section{Sharp Threshold for Connectivity}

The first lecture will be a proof of the following result. This proof uses several techniques you learned in this class.

\begin{theorembox}{Erdos-Renyi 1961}{}
Consider a graph $g \sim G(n, p(n))$ where $p(n) = \lambda \frac{\ln(n)}{n}$. Then as $n \rightarrow \infty$,
\begin{align*}
	P(g \text{ connected}) \rightarrow 0 & \quad \text{if } \lambda < 1\\
	P(g \text{ connected}) \rightarrow 1 & \quad \text{if } \lambda > 1
\end{align*}
\end{theorembox}

\begin{proof}
Suppose $\lambda < 1$. Since $P(\text{connected}) = 1 - P(\text{disconnected})$, we will show $P(\text{disconnected}) \rightarrow 1$ by showing that \textbf{there is at least 1 isolated node}. Define
\begin{itemize}
	\item $X_n$ to be a random variable that counts the number of isolated nodes
	\item $I_i$ to be a (Bernoulli) indicator random variable such that $I_i = 1$ when node $i$ is isolated and is $0$ otherwise
	\item Let $p = p(n)$ and $q = q(n) = (1 - p(n))^{n - 1}$ be  the probability of a node being isolated
\end{itemize}
We want to show $P(X_n > 0) \rightarrow 1$, or equivalently, $P(X_n = 0) \rightarrow 0$. To get a bound on $P(X_n = 0)$, we observe:
\begin{align*}
	\Var(X_n) 
	&= E\left(X_n - E(X_n)\right)\\
	&= P(X_n = 0)(0 - E(X_n)^2 + P(X_n = 1)(1 - E(X_n))^2 + ...\\
	&\ge P(X_n = 0)E(X_n)^2.
\end{align*}
Thus 
\begin{align}\label{claim1}
\frac{\Var(X_n)}{E(X_n)^2} \ge P(X_n=0). 
\end{align}
We will now calculate $\Var(X_n)$ and $E(X_n)$ explicitly to show that the left hand side of \eqref{claim1} goes to 0. By linearity of expectation and applying definition of indicators,
\begin{align*}
	E(X_n) = E\left(\sum_{i=1}^n I_i\right) = \sum_{i=1}^nE(I_i) = \sum_{i=1}^nP(I_i) = nq.
\end{align*}
Since indicators $I_i$ are \textbf{not independent} (why?), we use equation (1.10) in your book \cite{lange2010applied}:
\begin{align*}
	\Var(X_n) 
	&= \Var\left(\sum_{i=1}^nI_i\right) = \sum_{i=1}^n\Var(I_i) + \sum_{i=1}^n\sum_{j\neq i} \Cov(I_i, I_j)\\
	&= \sum_{i=1}^n q(1-q) + \sum_{i=1}^n \sum_{j\neq i}\left[ E(I_iI_j) - E(I_i)E(I_j) \right] \quad (\text{since Var(Bernoulli)} = p(1-p))\\
	&= nq(1-q) + \sum_{i=1}^n \sum_{j\neq i}\left[ P(I_i \cap I_j) - P(I_i)P(I_j) \right]\\
	&= nq(1-q) + \sum_{i=1}^n\sum_{j\neq i}\left[ (1-p)^{n-1}(1-p)^{n-2} - (1-p)^{n-1}(1-p)^{n-1} \right]\\
	&= nq(1-q) + \sum_{i=1}^n\sum_{j\neq i}\left[ \frac{q^2}{1-p} - q^2 \right]\\
	&= nq(1-q) + n(n-1)q^2\frac{p}{1-p}.
\end{align*}
Thus 
\begin{align*}
	\frac{\Var(X_n)}{E(X_n)^2} 
	&= \frac{nq(1-q) + n(n-1)q^2\frac{p}{1-p}}{(nq)^2} = \frac{1-q}{nq} + \frac{n-1}{n}\frac{p}{1-p}.
\end{align*}
We will now show these terms approach 0 as $n \rightarrow \infty$, then eq \eqref{claim1} will give us what we need.
The first term is dominated by $nq$, and
\begin{align*}
	\lim_{n \rightarrow \infty} nq 
	&= \lim_{n \rightarrow \infty} n(1-p)^{n-1} = \lim_{n \rightarrow \infty}  \exp \left\{ \ln(n) + (n-1)\ln(1 - p) \right\}\\
	&= \lim_{n \rightarrow \infty} \exp \left\{ \ln(n) + (n-1)\ln\left( 1 - \frac{\lambda \ln(n)}{n} \right) \right\}\\
	&\approx \lim_{n \rightarrow \infty} \exp \left\{ \ln(n) - \lambda\frac{n-1}{n}\ln(n) \right\} \quad (\ln(1 - x) = 1 - x + \frac{x^2}{2}- ... \approx -x + O(x^2) \text{ for small }x)\\
	&= \lim_{n \rightarrow \infty} \exp \left\{ \ln(n)\left( 1 - \lambda\frac{n-1}{n} \right) \right\}\\
	&= \infty \qquad \left(\text{since } \lambda < 1 \text{ and } n \rightarrow \infty \right)
\end{align*}
For the second term, observe that $p = \lambda \frac{\ln(n)}{n} \rightarrow 0$ as $n \rightarrow \infty$. So $\frac{p}{1-p} \rightarrow 0$ as well. This completes the case for $\lambda < 1$. \\
\\
\textbf{Part II.} Now suppose $\lambda > 1$. We want to show $P(\text{connected})\rightarrow 1,$ or equivalently $P(\text{disconnected})\rightarrow 0$. A graph is disconnected if there is a subgraph of $k$ nodes that does not connect to any of the other $n - k$ nodes (draw a picture). By symmetry, we only have to consider $k \in \{1, 2, ... \lfloor n/2 \rfloor\}$.  So 
\begin{align*}
	P(\text{disconnected}) 
	&= \bigcup_{k=1}^{\lfloor n/2 \rfloor} P(\text{some set of } k \text{ nodes not connected to the rest})\\
	&\le \sum_{k=1}^{\lfloor n/2 \rfloor} P(\text{some set of } k \text{ nodes not connected to the rest}) \quad (\text{inclusion-exclusion picture})\\
	&= \sum_{k=1}^{\lfloor n/2 \rfloor} {n \choose k} \left[ (1-p)^{(n - k)} \right]^k\\
	&\le \sum_{k=1}^{\lfloor n/2 \rfloor} {n \choose k} e^{p(n-k)k} \quad \left(e^{-x} = 1 - x + \frac{x^2}{2} - ... \approx 1 - x + O(x^2) \text{ for small }x\right)\\
	&= \sum_{k=1}^{\lfloor n/2 \rfloor} {n \choose k} \exp\left\{\frac{-\lambda \ln(n)(n-k)k}{n}\right\}\\
	&= \sum_{k=1}^{\lfloor n/2 \rfloor} {n \choose k} n^{\frac{-\lambda}{n}(n-k)k}\\
	&= \sum_{k=1}^{n^*} {n \choose k} n^{\frac{-\lambda}{n}(n-k)k} + \sum_{k=n^* + 1}^{\lfloor n/2 \rfloor} {n \choose k} n^{\frac{-\lambda}{n}(n-k)k} \quad \left(\text{Choose } n^* s.t. \frac{\lambda(n - n^*)}{n}>1 \iff n^* = \lfloor n(1 - \frac{1}{\lambda}) \rfloor\right)
\end{align*}
For the first term, 
\begin{align*}
	\sum_{k=1}^{n^*} {n \choose k} n^{\frac{-\lambda}{n}(n-k)k}
	&\le \sum_{k=1}^{n^*} n^k n^{\frac{-\lambda}{n}(n-k)k} = \sum_{k=1}^{n^*} \left[ n^{1 - \frac{\lambda}{n}(n-k)} \right]^k\\
	&\le \sum_{k=1}^{n^*} \left[ n^{1 - \frac{\lambda}{n}(n-n^*)} \right]^k \qquad \left(\text{judiciously bound inner} k \text{ with something bigger}\right)\\
	&= \sum_{k=1}^{n^*} r^k \qquad \left(\text{define } r = n^{1 - \frac{\lambda}{n}(n-n^*)}\right)\\
	&= \left(\sum_{k=0}^{n^*} r^k\right) - 1\\
	&= \frac{r}{1-r} \qquad (\text{geometric series; } 1 - \frac{\lambda}{n}(n-n^*) < 0, \text{ so } r < 1)\\
	&= \frac{1}{n^{\frac{\lambda}{n}(n-n^*) - 1} - 1}\\
	&\longrightarrow 0 \qquad \left(\text{since } n \rightarrow \infty \text{ and exponent} > 0\right)
\end{align*}
For the second term, we use a better bound than before (see homework):
\begin{align*}
	{n \choose k} < \left(\frac{ek}{k}\right)^k.
\end{align*}
Thus 
\begin{align*}
	\sum_{k=n^* + 1}^{\lfloor n/2 \rfloor} {n \choose k} n^{\frac{-\lambda}{n}(n-k)k} 
	&\le \sum_{k=n^* + 1}^{\lfloor n/2 \rfloor} \left(\frac{en}{k}\right)^k n^{\frac{-\lambda(n-k)k}{n}} = \sum_{k=n^* + 1}^{\lfloor n/2 \rfloor} \left[ \frac{en^{1 - \frac{\lambda(n-k)}{n}}}{k}\right]^k\\
	&\le \sum_{k=n^* + 1}^{\lfloor n/2 \rfloor} \left[ \frac{en^{1-\frac{\lambda (n - \frac{n}{2})}{n}}}{n^* + 1}\right]^k \qquad (\text{bound inner } k \text{ with something from above})\\
	&= \sum_{k=n^* + 1}^{\lfloor n/2 \rfloor} \left[\frac{en^{1 - \frac{\lambda}{2}}}{n(1 - \frac{1}{\lambda}) + 1}\right]^k \le \sum_{k=n^* + 1}^{\lfloor n/2 \rfloor} \left[\frac{en^{\frac{-\lambda}{2}}}{1 - \frac{1}{\lambda}}\right]^k\\
	&\le \sum_{k=n^* + 1}^{\lfloor n/2 \rfloor}  r^k \qquad (r = \frac{en^{\frac{-\lambda}{2}}}{1 - \frac{1}{\lambda}}, 0 < r < 1 \text{ for large }n)\\
	&\le \sum_{k=n^* + 1}^{\infty}r^k  = \sum_{k=0}^{\infty}r^k - \sum_{k=n^* + 1}^{n^*}r^k\\
	&= \frac{1}{1-r} - \frac{1-r^{n^*+1}}{1-r} \qquad (\text{finite geometric series} \sum_{k=0}^{m}r^k = \frac{1-r^{m+1}}{1-r})\\
	&= \frac{r^{n^* + 1}}{1-r} \longrightarrow 0 \qquad \text{since } n^* \rightarrow \infty.
\end{align*}
\end{proof}

\section{Problems}

In honor of Ken Lange, you are required to do 2 problems. If you do more I will grade your top 2 problems. Every problem is worth the same number of points. If a problem has subproblems, each subproblem is worth the same number of points.

\begin{problembox}{Bounds of binomial coefficients}{}
For integers $n$ and $k$, prove the following inequalities
\begin{align*}
	\frac{n^k}{k^k} \le {n \choose k} \le \frac{n^k}{k!} < \left( \frac{ne}{k}\right)^k
\end{align*}
which is used in our proof for theorem 2.1. For the strict inequality, rewrite $\frac{n^k}{k!} = \left(\frac{n}{k}\right)^k \frac{k^k}{k!}$ and use Taylor expansion on $e^k$.
\end{problembox}

\bibliographystyle{apalike}
\bibliography{references}

\end{document}